modified consistency1, rBPFDecoder, rBPFEncoder

coq/model/rBPFDecoder.v
@@ -287,7 +287,7 @@ Definition rbpf_decoder (pc : nat) (l : list int64) : option bpf_instruction :=
       let src : nat := Z.to_nat (Int64.unsigned (decode_bpf data 12 4)) in
       let off : int16 := Int16.repr (Int64.signed (decode_bpf data 16 16)) in
       let imm : int := Int.repr (Int64.signed (decode_bpf data 32 32)) in
-      if Z.eqb (Byte.unsigned op) (Z.of_nat 0x18) then
+      if Z.eqb (Byte.unsigned op) 0x18%Z then
         match nth_error l (S pc) with
         | Some data2 =>
             let imm2 : int := Int.repr (Int64.signed (decode_bpf data2 32 32)) in
