coq/model/Consistency1.v
@@ -1,5 +1,5 @@
 From Coq Require Import ZArith List Lia.
-From compcert.lib Require Import Integers Maps.
+From compcert.lib Require Import Integers Maps Zbits.
 From compcert.common Require Import Memory AST.
 From bpf.model Require Import ebpf rBPFCommType rBPFSyntax.
 From bpf.model Require Import rBPFDecoder rBPFEncoder BitfieldLemma BinSolver.
@@ -41,13 +41,104 @@ Ltac bin_solver :=
 
 Ltac unfold_bin := unfold binary_to_int64, decode_bpf, encode_bpf.
 
-Lemma int64_size_int_sign_le32: forall i,
-  Int64.size (Int64.repr (Int.signed i)) <= 32.
-Admitted.
+Lemma int64_size_int_unsign_le32: forall i,
+  Int64.size (Int64.repr (Int.unsigned i)) <= 32.
+Proof.
+  intros.
+  apply Int64.bits_size_3; [lia |].
+  intros n Hrange.
+  rewrite Int64.testbit_repr; [| lia].
+  apply Ztestbit_above with (n := 32%nat); [| lia].
+  unfold two_power_nat; simpl.
+  apply Int.unsigned_range.
+Qed.
 
-Global Hint Resolve int64_size_int_sign_le32 : int_size.
+Lemma int64_size_int16_unsign_le16: forall i,
+  Int64.size (Int64.repr (Int16.unsigned i)) <= 16.
+Proof.
+  intros.
+  apply Int64.bits_size_3; [lia |].
+  intros n Hrange.
+  rewrite Int64.testbit_repr; [| lia].
+  apply Ztestbit_above with (n := 16%nat); [| lia].
+  unfold two_power_nat; simpl.
+  apply Int16.unsigned_range.
+Qed.
+  
+
+Global Hint Resolve int64_size_int_unsign_le32 : int_size.
+Global Hint Resolve int64_size_int16_unsign_le16 : int16_size.
 
 Ltac bsolver := unfold_bin; simpl; repeat bin_solver; auto with int_size.
+
+
+Lemma int64_range_int_range_sign_le: forall i,
+  Int64.min_signed <= Int.unsigned i <= Int64.max_signed.
+Proof.
+  intros.
+  pose proof Int.unsigned_range i as Hrange.
+  destruct Hrange as [H1 H2].
+  split.
+  - rewrite <- H1.
+    unfold Int64.min_signed.
+    simpl.
+    lia.
+  - unfold Int64.max_signed, Int.modulus, two_power_nat in *.
+    simpl in *.
+    lia.
+Qed.
+  
+
+Lemma bpf_ireg_nat_trans_cons : forall b,
+  nat_to_bpf_ireg 
+    (Z.to_nat 
+      (Int64.unsigned 
+        (Int64.repr 
+          (Z.of_nat 
+            (bpf_ireg_to_nat b))))) = Some b.
+Proof.
+  unfold bpf_ireg_to_nat, nat_to_bpf_ireg.
+  destruct b; rewrite Int64.unsigned_repr; simpl;
+  try reflexivity; change Int64.max_unsigned with 18446744073709551615; lia.
+Qed.
+
+Lemma int_repr_int64_repr_cons : forall i, 
+  Int.repr (Int64.signed (Int64.repr (Int.unsigned i))) = i.
+Proof.
+  intros i.
+  rewrite Int64.signed_repr. 
+  - rewrite Int.repr_unsigned.
+    reflexivity.
+  - apply int64_range_int_range_sign_le.
+Qed.
+
+Lemma simple_memory_op : forall m,
+  Byte.unsigned
+      (Byte.repr
+         (Int64.unsigned
+            (Int64.repr
+               (Byte.unsigned
+                  (Byte.repr
+                     match m with
+                     | Mint8unsigned => 113
+                     | Mint16unsigned => 105
+                     | Mint32 => 97
+                     | Mint64 => 121
+                     | _ => 0
+                     end))))) = ( match m with
+                                | Mint8unsigned => 113
+                                | Mint16unsigned => 105
+                                | Mint32 => 97
+                                | Mint64 => 121
+                                | _ => 0
+                                end).
+Proof.
+  intros.
+  destruct m; 
+  try (rewrite Byte.unsigned_repr; rewrite Int64.unsigned_repr; rewrite Byte.unsigned_repr;
+       try ( unfold Byte.max_unsigned, Int64.max_unsigned; simpl; lia) 
+  ).
+Qed.
 
 Lemma rbpf_encode_decode_consistency:
   forall l_bin pc l ins
@@ -71,7 +162,110 @@ Proof.
     change (Byte.unsigned (Byte.repr (Int64.unsigned (Int64.repr (Byte.unsigned (Byte.repr 24))))) =? 24) with true.
     simpl.
     rewrite Hnth0.
-    + bsolver. (*TODO
+    + bsolver.
+      rewrite bpf_ireg_nat_trans_cons.
+      rewrite int_repr_int64_repr_cons.
+      rewrite int_repr_int64_repr_cons.
+      reflexivity.
+    + fold Int64.zero.
+      rewrite Int64.size_zero.
+      lia.
+    + unfold Int64.size.
+      rewrite Int64.unsigned_repr.
+      * unfold Zsize.
+        lia.
+      * unfold Int64.max_unsigned.
+        simpl.
+        lia.
+    + destruct b;
+      try ( simpl; unfold Int64.size, Zsize; rewrite Int64.unsigned_repr;
+      [ simpl; lia | unfold Int64.max_unsigned; simpl; lia ] ).
+    + rewrite Byte.unsigned_repr.
+      * unfold Int64.size.
+        rewrite Int64.unsigned_repr.
+        -- unfold Zsize.
+           simpl.
+           lia.
+        -- unfold Int64.max_unsigned.
+           simpl.
+           lia.
+      * unfold Byte.max_unsigned.
+        simpl.
+        lia.
+  - destruct nth_error as [ins |] eqn: Hnth; [| inversion HL].
+    rewrite Bool.andb_true_iff in HL.
+    destruct HL as (Hins & HL).
+    destruct l as [| h0 l0]; [inversion HL |].
+    destruct nth_error as [ins0 |] in HL; [| inversion HL].
+    rewrite Bool.andb_true_iff in HL.
+    destruct HL as (Hins0 & _).
+    apply Int64.same_if_eq in Hins, Hins0.
+    unfold rbpf_decoder_one.
+    subst.
+    bsolver.
+    rewrite simple_memory_op.
+    destruct m; simpl.
+    + rewrite bpf_ireg_nat_trans_cons.
+      rewrite bpf_ireg_nat_trans_cons.
+
+
+
+
+
+      bsolver.
+      reflexivity.
+    + fold Int64.zero.
+      rewrite Int64.size_zero.
+      lia.
+    + unfold Int64.size.
+      rewrite Int64.unsigned_repr.
+      * unfold Zsize.
+        lia.
+      * unfold Int64.max_unsigned.
+        simpl.
+        lia.
+    + destruct b;
+      try ( simpl; unfold Int64.size, Zsize; rewrite Int64.unsigned_repr;
+      [ simpl; lia | unfold Int64.max_unsigned; simpl; lia ] ).
+    + rewrite Byte.unsigned_repr.
+      * unfold Int64.size.
+        rewrite Int64.unsigned_repr.
+        -- unfold Zsize.
+           simpl.
+           lia.
+        -- unfold Int64.max_unsigned.
+           simpl.
+           lia.
+      * unfold Byte.max_unsigned.
+        simpl.
+        lia.
+
+      
+
+ simpl; unfold Int64.size, Zsize; rewrite Int64.unsigned_repr; 
+      [ lia | unfold Int64.max_unsigned; simpl; lia ].
+
+
+apply Int64.bits_size_3; [lia |].
+      intros n Hrange.
+      rewrite Int64.testbit_repr; [| lia].
+      apply Ztestbit_above with (n := (bpf_ireg_to_nat b)).
+      * unfold two_power_nat; simpl.
+        destruct b; simpl; lia.
+      * destruct b; simpl.
+        -- destruct Hrange as [Hlow Hhigh].
+           try lia.
+        -- 
+
+
+        
+      
+      match goal with
+      | |- context[Int64.unsigned_bitfield_extract ?p0 ?w0 (Int64.bitfield_insert ?p0 ?w0 ?i0 ?v0)] =>
+           erewrite unsigned_bitfield_extract_bitfield_insert_same_1 with (pos := p0) (width := w0)
+  end.
+
+ (*
   match goal with
 
 
